Earley/Proofs/Parser.lean
@@ -77,7 +77,7 @@ public theorem soundnessParse {G : ContextFreeGrammar T} [BEq G.NT] [LawfulBEq G
     simp only [recognizeList, decide_eq_true_eq]
     use x.item
     let finalBin := (earleyList Gₗ w).bins[w.length]
-    let P := fun x : BinItem T G.NT => isFinished Gₗ.initial (mapT w) x.item
+    let P := fun x : BinItem T G.NT => isFinished Gₗ.initial w.length x.item
     have hmem : (x, idx) ∈ (filterWithIdx finalBin P) := by grind
     have := P_of_filterWithIdx finalBin P hmem
     have := getElem_of_filterWithIdx finalBin P hmem
@@ -159,7 +159,7 @@ public theorem completenessParse {G : ContextFreeGrammar T} [BEq G.NT] [LawfulBE
   split
   · rename_i heq
     rcases this with ⟨x,hx⟩
-    let P := fun y : EarleyItem T G.NT => isFinished Gₗ.initial (mapT w) y
+    let P := fun y : EarleyItem T G.NT => isFinished Gₗ.initial w.length y
     grind [notP_of_emptyFilterWithIdx]
   · rename_i x idx bins hf
     apply some_of_buildTree Gₗ w idx
